LeanProjeto2/Technicalities.lean
@@ -1,2 +1,2 @@
 import LeanProjeto2.FOL
-import LeanProjeto2.StarLang
+import LeanProjeto2.StarLang_old
